\documentclass[11pt]{beamer}
\usepackage{amsfonts,amsmath,amsthm,amssymb}
\theoremstyle{plain}
\newtheorem{conjecture}{Conjecture}[section]
\usepackage{mathtools,mathptmx,listings,forest,enumitem}
\usepackage{graphicx}
\usepackage{pgfplots}
\pgfplotsset{compat=newest}
% plotting things
\usepackage{graphicx}
% \graphicspath{{images/}}
\graphicspath{{../}}
\usepackage{tikz-cd}
\pgfplotsset{compat=1.15}
\usepackage[
	backend=biber,
	style=verbose,
	sorting=ynt
]{biblatex}
\addbibresource{references.bib}
\usetheme{Madrid}
\usepackage{float,mathtools,dirtytalk,ulem,csquotes,cancel,hyperref}
\author[] % (optional)
{Emon Hossain\inst{1}}

\institute[University of Dhaka] % (optional)
{
  \inst{1}%
  Lecturer\\MNS department\\Brac University
}

\date[] % (optional)
{\textsc{Lecture-05}}


\title[]{MAT215: Complex Variables And Laplace Transformations}

\setbeamertemplate{navigation symbols}{}


\AtBeginSection[]
{
  \begin{frame}
    \frametitle{Table of Contents}
    \tableofcontents[currentsection]
  \end{frame}
}

\usepackage{Kyushu}

% \usetheme{Frankfurt}

\begin{document}
\begin{frame}
\titlepage
\end{frame}

\begin{frame}{Derivative formula}
    \begin{example}
        Show that, $$\mathcal{L}\{y'(t)\}=sY(s)-y(0)$$
    \end{example}
    \begin{example}
        Show that, $$\mathcal{L}\{y''(t)\}=s^2Y(s)-sy(0)-y'(0)$$
    \end{example}
    \begin{example}
        Show that, $$\mathcal{L}\{y'''(t)\}=s^3Y(s)-s^2y(0)-sy'(0)-y''(0)$$
    \end{example}
\end{frame}

\begin{frame}{Example}
    \begin{example}
        Solve the given differential equation:
        $$y''-4y'+4y=t^3e^{2t},\:y(0)=0,y'(0)=0$$
    \end{example}
    \begin{example}
        Solve the given differential equation:
        $$y''-3y'+2y=4,y(0)=1,y'(0)=-1$$
        \textbf{Hint:}
        $$\frac{s-2}{s(s-1)}=\frac{2}{s}+\frac{-1}{s-1}$$
    \end{example}
\end{frame}
\begin{frame}{Example}
    \begin{example}
        Solve the given differential equation:
        $$y'''-3y''+3y'-y=e^t t^2,\:y(0)=0,y'(0)=1,y''(0)=-2$$
    \end{example}
    \begin{example}
        Solve the given differential equation:
        $$\frac{dy}{dt}+y=13\sin 2t,\:y(0)=6$$
        \textbf{Hint:}
        $$\frac{6s^2+50}{(s+3)(s^2+4)}=\frac{8}{(s+3)}+\frac{-2s+6}{(s^2+4)}$$
    \end{example}
\end{frame}
\end{document}