\documentclass[11pt]{beamer}
\usepackage{amsfonts,amsmath,amsthm,amssymb}
\theoremstyle{plain}
\newtheorem{conjecture}{Conjecture}[section]
\usepackage{mathtools,mathptmx,listings,forest,enumitem}
\usepackage{graphicx}
\usepackage{pgfplots}
\pgfplotsset{compat=newest}
% plotting things
\usepackage{graphicx}
% \graphicspath{{images/}}
\graphicspath{{../}}
\usepackage{tikz-cd}
\pgfplotsset{compat=1.15}
\usepackage[
	backend=biber,
	style=verbose,
	sorting=ynt
]{biblatex}
\addbibresource{references.bib}
\usetheme{Madrid}
\usepackage{float,mathtools,dirtytalk,ulem,csquotes,cancel,hyperref}
\author[] % (optional)
{Emon Hossain\inst{1}}

\institute[University of Dhaka] % (optional)
{
  \inst{1}%
  Lecturer\\MNS department\\Brac University
}

\date[] % (optional)
{\textsc{Lecture-02}}


\title[]{MAT215: Complex Variables And Laplace Transformations}

\setbeamertemplate{navigation symbols}{}


\AtBeginSection[]
{
  \begin{frame}
    \frametitle{Table of Contents}
    \tableofcontents[currentsection]
  \end{frame}
}

\usepackage{Kyushu}

% \usetheme{Frankfurt}

\begin{document}
\begin{frame}
\titlepage
\end{frame}

\begin{frame}
    \frametitle{Some important formulas}
    $$
    2 \sin(A)\cos(B)=\sin(A+B)+\sin(A-B)
    $$
    $$
    2 \cos(A)\cos(B)=\cos(A+B)+\cos(A-B)
    $$
    $$
    2 \sin(A)\sin(B)=\cos(A-B)-\cos(A+B)
    $$

    $$\sinh (\theta) =\frac{e^\theta- e^{-\theta}}{2}, \cosh (\theta) =\frac{e^\theta+ e^{-\theta}}{2}$$

    $$
    \int e^{at}\sin(bt)dt=\frac{e^{at}}{a^2+b^2}(a\sin(bt)-b\cos(bt))+C
    $$
    $$\int e^{at}\cos(bt)dt=\frac{e^{at}}{a^2+b^2}(a\cos(bt)+b\sin(bt))+C$$
\end{frame}

\begin{frame}
    \frametitle{Some important Laplace Transform formulas}
     \begin{itemize}[label=$\bullet$]
    \item Known formula 
    \item First Translation formula:
    $$\boxed{\mathcal L\{e^{at}f(t)\}=\mathcal L\{f(t)\}_{s\rightarrow s-a}=F(s-a)}$$
    % $$
    % \boxed{\underbrace{\mathcal L^{-1}\{F(s)\}}_{\text{unknown}}=e^{at}\underbrace{\mathcal L^{-1}\{F(s+a)\}}_{\text{known}}}
    % $$
    \item Truncation/Second Translation formula:
    $$\boxed{\mathcal{L}\{f(t-a)u(t-a)\}=e^{-as}F(s)}$$
    % $$\boxed{\mathcal{L}^{-1}\{F(s)e^{-as}\}=f(t-a)u(t-a)}$$
    \item $s$-differentiation:
    $$\boxed{\mathcal{L}\{(t)^nf(t)\}=(-1)^n\frac{d^n}{ds^n}F(s)}$$  
    \item Partial fraction type
    \item Convolution type (Not very important)
\end{itemize}
\end{frame}

\begin{frame}
    \frametitle{Example}
    \begin{example}
        Find the Laplace transform of $f(t)=t$.
    \end{example}
    \begin{example}
        Find the Laplace transform of $f(t)=e^{at}$.
    \end{example}
\begin{example}
        \begin{enumerate}[label=\alph*.]
            \item Find the Laplace transform of $f(t)= 2e^{-2t}$.
            \item Find the Laplace transform of $f(t)= 4t^3-e^{-1}$.
            \item Find the Laplace transform of $f(t)= (t^2+1)^2$.
            \item Find the Laplace transform of $f(t)= \cosh(3t)+\sin(2t)$.
        \end{enumerate}
    \end{example}
\end{frame}


\begin{frame}
        \begin{example}
        \begin{enumerate}[label=\alph*.] 
            \item Find the Laplace transform of $f(t)=\cos(at)$.
            \item Find the Laplace transform of $f(t)=\sin(at)$.
            \item Find the Laplace transform of $f(t)=\sinh(at)$.
            \item Find the Laplace transform of $f(t)=\cosh(at)$.
        \end{enumerate}
    \end{example}
\end{frame}


\begin{frame}
    \frametitle{Way-01}
    Find the Laplace transform of $f(t)=\sin(at)$.
    \begin{align*}
        \mathcal L\{\sin(at)\} &=\int_0^\infty e^{-st}\sin(at)dt\\
        &= \text{Skip way-01} 
    \end{align*}
\end{frame}

\begin{frame}
    \frametitle{Way-02 (best way)}
    Find the Laplace transform of $f(t)=\sin(at)$.
    \begin{align*}
        \mathcal L\{\sin(at)\} &=\int_0^\infty e^{-st}\sin(at)dt \\
        &= \int_0^\infty e^{-st} \frac{e^{i(at)}-e^{-i(at)}}{2i} dt\\
        &= \frac{1}{2i}\left(\int_0^\infty e^{-st} e^{i(at)} dt - \int_0^\infty e^{-st} e^{-i(at)} dt\right) \\
        &= \frac{1}{2i} \left[ \frac{1}{s-ia} - \frac{1}{s+ia} \right]\\
        &=  \frac{1}{2i} \frac{2i a}{s^2 + a^2}\\
        &= \frac{a}{s^2 + a^2}
    \end{align*}
\end{frame}


\begin{frame}
    \frametitle{Way-03}
    Find the Laplace transform of $f(t)=\sin(at)$.
    \begin{align*}
        \mathcal L\{\sin(at)\} &=\int_0^\infty e^{-st}\sin(at)dt \\
        &=\lim_{b\to\infty}\int_0^b e^{-st}\sin(at)dt \\
        &=\lim_{b\to\infty}\left[\frac{e^{-st}(-a\cos(at)-s\sin(at))}{a^2+s^2}\right]_0^b \\
        &=\lim_{b\to\infty}\left(\frac{e^{-sb}(-a\cos(ab)-s\sin(ab))}{a^2+s^2}-\frac{-a}{a^2+s^2}\right) \\
        &=\frac{a}{a^2+s^2}
    \end{align*}
\end{frame}


\begin{frame}
    \begin{example}
        \begin{itemize}[label=$\bullet$]
            \item Find the Laplace transform of $f(t)=t^3$.
            \item Find the Laplace transform of $f(t)=t^3 e^{5t}$.
            \text{Hint: Use the first Translation formula:}
            $$\boxed{\mathcal L\{e^{at}f(t)\}=\mathcal L\{f(t)\}_{s\rightarrow s-a}=F(s-a)}$$
        \end{itemize}
    \end{example}
    \begin{example}
        \begin{itemize}
            \item Find the Laplace transform of $f(t)=5\sin(4t)$.
            \item Find the Laplace transform of $f(t)=5\sin(4t) e^{-3t}$.
            \text{Hint: Use the first Translation formula:}
            $$\boxed{\mathcal L\{e^{at}f(t)\}=\mathcal L\{f(t)\}_{s\rightarrow s-a}=F(s-a)}$$
        \end{itemize}
    \end{example}
\end{frame}

\begin{frame}
    \begin{example}
        \begin{itemize}
            \item Find the Laplace transform of $f(t)=(t+2)^2$.
            \item Find the Laplace transform of $f(t)=(t+2)^2 e^t$.
        \end{itemize}
    \end{example}
\end{frame}

\begin{frame}
    \begin{example}
        \begin{itemize}
            \item Find the Laplace transform of $f(t)=t\sin(at)$.
        \end{itemize}
    \end{example}
        \pause
            \begin{align*}
                \mathcal L\{t\sin(at)\} &= \int_0^\infty e^{-st}t\sin(at)dt \\
                &= \int_0^\infty t \underbrace{e^{-st} \sin(at)}_{v} dt\\
                &= \left[ t \frac{e^{-st}(-a\cos(at)-s\sin(at))}{a^2+s^2} \right]_0^\infty \\
                & \qquad - \int_0^\infty \left[ t \frac{e^{-st}(-a\cos(at)-s\sin(at))}{a^2+s^2} \right]_0^\infty dt\\
                &= \frac{s}{(s^2+a^2)} \int_0^\infty e^{-st}\sin(at)dt + \frac{a}{(s^2+a^2)} \int_0^\infty e^{-st}\cos(at)dt \\
                &= \frac{s}{(s^2+a^2)} \cdot \frac{a}{s^2+a^2} + \frac{a}{(s^2+a^2)} \cdot \frac{s}{s^2+a^2} \\
                &= \frac{2as}{(s^2+a^2)^2}
            \end{align*}
\end{frame}

\begin{frame}
    \frametitle{Way-02}
    \textbf{Solution:}
    \begin{align*}
        \mathcal L\{t\sin(at)\} &= \int_0^\infty e^{-st}t\sin(at)dt \\
        &= -\int_0^\infty e^{-st} \frac{\partial}{\partial a} \left( \cos(at) \right) dt\\
        &= - \frac{\partial}{\partial a} \int_0^\infty e^{-st} \cos(at) dt \\
        &= - \frac{\partial}{\partial a} \left( \frac{s}{s^2 + a^2} \right) \\
        &= \frac{2as}{(s^2 + a^2)^2}
    \end{align*}
\end{frame}

\begin{frame}
    \begin{example}
        \begin{itemize}
            \item Find the Laplace transform of $f(t)=2\sinh(3t)+5\cosh(4t)$.
            \item Find the Laplace transform of $f(t)=e^{2t}[2\sinh(3t)+5\cosh(4t)]$.
            \item Find the Laplace transform of $f(t)=t e^{2t}[2\sinh(3t)+5\cosh(4t)]$
        \end{itemize}
    \end{example}
\end{frame}


\end{document}